snap

state/TargetLang.fst
@@ -1,5 +1,6 @@
 module TargetLang
 
+open FStar.Ghost
 open FStar.Tactics
 open FStar.Tactics.Typeclasses
 open FStar.Ref
@@ -8,7 +9,7 @@ type tfootprint = Set.set nat
 
 (** target_lang is a shallow embedding of STLC **)
 class target_lang (t:Type) = {
-    footprint : t -> heap -> GTot tfootprint
+    footprint : t -> heap -> (erased tfootprint)
 }
 
 instance target_lang_unit : target_lang unit = {
@@ -50,9 +51,13 @@ let mk_tgt_arrow
   x:t1 -> ST (t2 x) 
      (requires (fun _ -> True))
      (ensures (fun h0 r h1 -> 
-        let fp = (target_lang_pair tscope t1).footprint (scope, x) h0 in
-        (modifies fp h0 h1) /\
-        (forall z. Set.mem z ((c2 x).footprint r h1) ==> Set.mem z fp \/ addr_unused_in z h0) // <-- returned references either are already in scope or are fresh
+        let fp0 = (target_lang_pair tscope t1).footprint (scope, x) h0 in
+     //    let fp1 = (target_lang_pair tscope t1).footprint (scope, x) h1 in
+        (modifies fp0 h0 h1)
+     //    (exists fp1' fp1''. Set.disjoint fp1' fp1'' /\ Set.equal fp1 (Set.union fp1' fp1'') /\
+     //                        fp1' `Set.subset` fp0 /\ (forall ad. ad `Set.mem` fp1'' ==> addr_unused_in ad h0))
+         ///\
+     //    (forall z. Set.mem z ((c2 x).footprint r h1) ==> Set.mem z fp \/ addr_unused_in z h0) // <-- returned references either are already in scope or are fresh
  ))
 
 instance target_lang_arrow 
@@ -64,8 +69,8 @@ instance target_lang_arrow
     {| target_lang tscope |}
     {| (x:t1 -> target_lang (t2 x)) |}
     : 
-    target_lang (mk_tgt_arrow t1 t2 scope)  = {
-    footprint = fun _ _ -> Set.empty
+    target_lang (mk_tgt_arrow t1 t2 scope) = {
+    footprint = fun _ _ -> Set.empty           // <-- TODO: why no footprint for functions?
 }
 
 open STLC
@@ -97,6 +102,9 @@ let rec elab_typ' (t:typ) (#tscope:Type) (scope:tscope) (c_scope:target_lang tsc
 let elab_typ (t:typ) : Type =
   dfst (elab_typ' t () target_lang_unit)
 
+let elab_typ_footprint (t:typ) =
+  dsnd (elab_typ' t () target_lang_unit)
+
 val elab_typ_test1 : elab_typ (TArr (TRef (TRef TNat)) (TArr (TRef TNat) TUnit))
 let elab_typ_test1 (x:ref (ref int)) (y:ref int) =
   let ix = !x in
@@ -111,8 +119,119 @@ let elab_typ_test2 () = alloc 0
 val elab_typ_test2' : elab_typ (TArr (TRef TNat) (TRef TNat))
 let elab_typ_test2' x = x
 
-val elab_typ_test3 : elab_typ (TArr (TArr TUnit (TRef TNat)) TUnit)
-let elab_typ_test3 f =
-  let x:ref int = f () in
-  x := !x + 1;
-  ()
+// val elab_typ_test3 : elab_typ (TArr (TArr TUnit (TRef TNat)) TUnit)
+// let elab_typ_test3 f =
+//   let x:ref int = f () in
+//   x := !x + 1;
+//   ()
+
+(*** NOT UPDATED FROM HERE **)
+(** *** Elaboration of expressions to F* *)
+type vcontext (g:context) = x:var{Some? (g x)} -> elab_typ (Some?.v (g x))
+
+let vempty : vcontext empty = fun _ -> assert false
+
+let vextend #t (x:elab_typ t) (#g:context) (ve:vcontext g) : vcontext (extend t g) =
+  fun y -> if y = 0 then x else ve (y-1)
+
+
+//let cast_TArr #t1 #t2 (h : (elab_typ t1 -> Tot (elab_typ t2))) : elab_typ (TArr t1 t2) = h
+
+open FStar.List.Tot
+
+// let rec fnrec (#a:Type) (n:nat) (acc:a) (iter:a -> a): Tot a =
+//      if n = 0 then acc else fnrec (n-1) (iter acc) iter
+
+let rec elab_exp 
+     (#g:context)
+     (#e:exp) 
+     (#t:typ)
+     (tyj:typing g e t)
+     (ve:vcontext g)
+     (#tscope:Type)
+     (scope:tscope)
+     {| sfp:target_lang tscope |}       
+  : ST (elab_typ t) 
+     (requires (fun _ -> True))
+     (ensures (fun h0 r h1 ->
+          let fp0 = sfp.footprint scope h0 in
+          let fp1 = sfp.footprint scope h1 in
+          (modifies fp0 h0 h1)))
+     (decreases e) = // <-- TODO: ST is divergent, can we state that this terminates?
+     // let h0 = gst_get () in
+     // let fp = sfp.footprint scope h0 in
+     match tyj with
+     | TyUnit -> ()
+     | TyZero -> 0
+     | TyAllocRef #_ #_ #t tyj_e -> begin
+          let v : elab_typ t = elab_exp tyj_e ve scope #sfp in
+          alloc v // <-- either this modifies the footprint or not
+     end
+     | TyReadRef #_ #_ #t tyj_e -> begin
+          let v : ref (elab_typ t) = elab_exp tyj_e ve scope #sfp in
+          read v
+     end
+     | TyWriteRef #_ #_ #_ #t tyj_ref tyj_v -> begin
+               let h0 = gst_get () in
+               let fp0 = sfp.footprint scope h0 in
+          let r : ref (elab_typ t) = elab_exp tyj_ref ve scope #sfp in // <-- this is effectful and modifies fp
+               let h1 = gst_get () in
+          let v : elab_typ t = elab_exp tyj_v ve scope #sfp in // this is effectul and modifies fp
+               let h2 = gst_get () in
+               assume (modifies fp0 h0 h2);
+          write r v;
+               let h3 = gst_get () in
+               assert (modifies (only r) h2 h3);
+               assume (Set.subset (only r) fp0);
+               assert (modifies fp0 h0 h3);
+          ()
+     end
+     | _ -> admit ()
+
+     (**
+     | TySucc hs ->
+          1 + (elab_exp hs ve)
+     | TyNRec h1 h2 h3 -> admit ()
+          // let v1 = elab_exp h1 ve in
+          // let v2 : elab_typ t = elab_exp h2 ve in
+          // let v3 : elab_typ (TArr t t) = elab_exp h3 ve in
+          // fnrec #(elab_typ t) v1 v2 v3
+     | TyInl #_ #_ #t1 #t2 h1 ->
+          let v = elab_exp h1 ve in
+          Inl #(elab_typ t1) #(elab_typ t2) v
+     | TyInr #_ #_ #t1 #t2 h1 ->
+          let v = elab_exp h1 ve in
+          Inr #(elab_typ t1) #(elab_typ t2) v
+     | TyCaseSum h1 h2 h3 ->
+          let v1 = elab_exp h1 ve in
+          let v2 = elab_exp h2 ve in
+          let v3 = elab_exp h3 ve in
+          (match v1 with | Inl x -> v2 x | Inr y -> v3 y)
+     | TyCaseNat h1 h2 h3 ->
+          let v1 = elab_exp h1 ve in
+          let v2 = elab_exp h2 ve in
+          let v3 = elab_exp h3 ve in
+          (match v1 with | 0 -> v2 () | _ -> v3 (v1-1))
+     | TyVar x -> ve x
+     | TyAbs t1 #_ #t2 h1 -> admit ()
+          // assert (t == TArr t1 t2);
+          // let w : elab_typ t1 -> Tot (elab_typ t2) =
+          // (fun x -> elab_exp h1 (vextend x ve)) in
+          // cast_TArr w
+     | TyApp #_ #_ #_ #t1 #t2 h1 h2 ->
+          assert ((elab_typ t) == (elab_typ t2));
+          (* TODO: Should we change the order here, first evaluate argument? *)
+          let v1 : elab_typ (TArr t1 t2) = elab_exp h1 ve in
+          let v2 : elab_typ t1 = elab_exp h2 ve in
+          v1 v2
+     | TyFst #_ #_ #t1 #t2 h1 ->
+          let v = elab_exp h1 ve in
+          fst #(elab_typ t1) #(elab_typ t2) v
+     | TySnd #_ #_ #t1 #t2 h1 ->
+          let v = elab_exp h1 ve in
+          snd #(elab_typ t1) #(elab_typ t2) v
+     | TyPair h1 h2 ->
+          let v1 = elab_exp h1 ve in
+          let v2 = elab_exp h2 ve in
+          (v1, v2)
+**)
